Clean up code and document current gap

src/api/dotnet/Client.cs
@@ -8,7 +8,7 @@ using Dafny;
 using ibyteseq = Dafny.ISequence<byte>;
 using icharseq = Dafny.ISequence<char>;
 using encryptioncontext = Dafny.Map<Dafny.ISequence<byte>, Dafny.ISequence<byte>>;
-using EncryptionStreams;
+using ESDKClientStreams;
 using Collections;
 using byteseq = Dafny.Sequence<byte>;
 using charseq = Dafny.Sequence<char>;
@@ -19,15 +19,39 @@ namespace AWSEncryptionSDK
     // TODO: What to name this?
     public class Client {
 
-        // TODO: Proper documentation
-        // TODO: should return some custom stream that "reads" the encryption
-        // ie it can't all be loaded into memory
-        public static EncryptionStream Encrypt(Stream plaintext, CMM cmm, Dictionary<string, string> encryptionContext = null, ushort? algorithmSuiteID = null, uint? frameLength = null) {
+        public static ClientEncryptionStream EncryptStream(Stream plaintext, CMM cmm, Dictionary<string, string> encryptionContext = null, ushort? algorithmSuiteID = null, uint? frameLength = null) {
             if (algorithmSuiteID != null && !AlgorithmSuite.__default.VALID__IDS.Elements.Contains((ushort)algorithmSuiteID)) {
                 throw new ArgumentException("Invalid algorithmSuiteID: " + algorithmSuiteID.ToString());
             }
-            ExternByteProducer input = new ExternByteProducer();
-            input.SetInputStream(plaintext);
+            // TTODO he way we handle this extern is weird. Determine if there
+            // is a clearer way to have an extern implement a Dafny trait, and then
+            // be usable in the shim layer.
+            InputStreamByteProducer input = new InputStreamByteProducer(plaintext);
+  
+             // TODO: This isn't checking for nulls or any of the requirements on the Dafny method.
+            // See https://github.com/dafny-lang/dafny/issues/461.
+            // TODO: Might need a lock here if ANYTHING in the Dafny runtime isn't threadsafe!
+            var optAlgorithmSuiteID = algorithmSuiteID != null ? STL.Option<ushort>.create_Some((ushort)algorithmSuiteID) : STL.Option<ushort>.create_None();
+            var optFrameLength = frameLength != null ? STL.Option<uint>.create_Some((uint)frameLength) : STL.Option<uint>.create_None();
+            var dafnyEncryptionContext = encryptionContext != null ? STL.Option<encryptioncontext>.create_Some(ToDafnyEncryptionContext(encryptionContext)) : STL.Option<encryptioncontext>.create_None();
+            
+            STL.Result<EncryptionStreams.EncryptionStream> result = ESDKClient.__default.StreamEncrypt(
+                    input,
+                    cmm,
+                    dafnyEncryptionContext,
+                    optAlgorithmSuiteID,
+                    optFrameLength
+            );
+
+            return new ClientEncryptionStream(DafnyFFI.ExtractResult(result));
+        }
+
+        // TODO: Proper documentation
+        public static MemoryStream Encrypt(MemoryStream plaintext, CMM cmm, Dictionary<string, string> encryptionContext = null, ushort? algorithmSuiteID = null, uint? frameLength = null) {
+            if (algorithmSuiteID != null && !AlgorithmSuite.__default.VALID__IDS.Elements.Contains((ushort)algorithmSuiteID)) {
+                throw new ArgumentException("Invalid algorithmSuiteID: " + algorithmSuiteID.ToString());
+            }
+            ibyteseq dafnyPlaintext = DafnyFFI.SequenceFromMemoryStream(plaintext);
     
             // TODO: This isn't checking for nulls or any of the requirements on the Dafny method.
             // See https://github.com/dafny-lang/dafny/issues/461.
@@ -35,24 +59,32 @@ namespace AWSEncryptionSDK
             var optAlgorithmSuiteID = algorithmSuiteID != null ? STL.Option<ushort>.create_Some((ushort)algorithmSuiteID) : STL.Option<ushort>.create_None();
             var optFrameLength = frameLength != null ? STL.Option<uint>.create_Some((uint)frameLength) : STL.Option<uint>.create_None();
             var dafnyEncryptionContext = encryptionContext != null ? STL.Option<encryptioncontext>.create_Some(ToDafnyEncryptionContext(encryptionContext)) : STL.Option<encryptioncontext>.create_None();
-            
-            // THese two shuould be encapsulated by one object in dafny
-            STL.Result<ESDKClient.EncryptorStream> result = ESDKClient.__default.StreamEncrypt(
-                    input,
+            STL.Result<ibyteseq> result = ESDKClient.__default.Encrypt(
+                    dafnyPlaintext,
                     cmm,
                     dafnyEncryptionContext,
                     optAlgorithmSuiteID,
                     optFrameLength
                     );
+    
+            return DafnyFFI.MemoryStreamFromSequence(DafnyFFI.ExtractResult(result));
+        }
 
-            return new EncryptionStream(DafnyFFI.ExtractResult(result));
+        // TODO: Currently just reading all of the input stream into memory, then
+        // doing the one shot Decrypt operation
+        public static MemoryStream StreamDecrypt(Stream cyphertext, CMM cmm) {
+            ibyteseq dafnyPlaintext = DafnyFFI.SequenceFromStream(cyphertext);
+    
+            // TODO: Might need a lock here if ANYTHING in the Dafny runtime isn't threadsafe!
+            STL.Result<ibyteseq> result = ESDKClient.__default.Decrypt(dafnyPlaintext, cmm);
+    
+            return DafnyFFI.MemoryStreamFromSequence(DafnyFFI.ExtractResult(result));
         }
   
         // TODO: Proper documentation
-        // TODO: should return some custom stream that "reads" the decryption
-        // ie it can't all be loaded into memory
-        public static MemoryStream Decrypt(Stream cyphertext, CMM cmm) {
-            ibyteseq dafnyPlaintext = DafnyFFI.SequenceFromStream(cyphertext);
+        public static MemoryStream Decrypt(MemoryStream cyphertext, CMM cmm) {
+            ibyteseq dafnyPlaintext = DafnyFFI.SequenceFromMemoryStream(cyphertext);
+    
             // TODO: Might need a lock here if ANYTHING in the Dafny runtime isn't threadsafe!
             STL.Result<ibyteseq> result = ESDKClient.__default.Decrypt(dafnyPlaintext, cmm);
     
