src/extern/dotnet/Collections.cs
@@ -4,34 +4,36 @@ using ESDKClient;
 using STL;
 
 namespace Collections {
-    public partial class ExternByteProducer {
+    public partial class InputStreamByteProducer {
         // TODO should be readonly, however we can't set in constructor due to
         // weird extern-ness
-        private Stream stream;
+        private Stream inputStream;
 
-        public void SetInputStream(Stream stream) {
-            this.stream = stream;
+        public InputStreamByteProducer(Stream inputStream) {
+            this.inputStream = inputStream;
         }
 
         // TODO ideally this shouldn't be used
         // and instead we rely on a more efficient way
-        // to read from the input stream
+        // to read from the input stream.
+        // i.e. There should be a Siphon that is able
+        // to make use of a more efficient read for C# read
         public Result<byte> ExternNext() {
             byte[] bytes = new byte[1];
-            stream.Read(bytes, 0, 1);
+            inputStream.Read(bytes, 0, 1);
             return Result<byte>.create_Success(bytes[0]);
         }
 
-        // TODO Need to assume that input stream is seekable.
-        // If it is not, then we need to load everything into memory?
-        // For now, just assume
+        // TODO Assumes that the input stream is seekable.
         public bool ExternHasNext() {
-            return stream.Position != stream.Length;
+            return inputStream.Position != inputStream.Length;
         }
         
+        // TODO Assumes that the input stream is seekable.
+        // Ideally, we shouldn't need the ByteProducer to expose this.
         public int Length() {
-            // TODO cutting off int sizes
-            return (int)stream.Length;
+            // TODO cutting off long sizes
+            return (int)inputStream.Length;
         }
     }
 }
