src/SDK/EncryptionStreams.dfy
@@ -1,0 +1,220 @@
+include "../StandardLibrary/StandardLibrary.dfy"
+include "../StandardLibrary/UInt.dfy"
+include "Materials.dfy"
+include "MessageHeader.dfy"
+include "MessageBody.dfy"
+include "Serialize.dfy"
+include "../Util/Streams.dfy"
+include "../Crypto/Signature.dfy"
+include "../StandardLibrary/Collections.dfy"
+
+module {:extern "EncryptionStreams"} EncryptionStreams {
+  import opened StandardLibrary
+  import opened UInt = StandardLibrary.UInt
+  import Materials
+  import AlgorithmSuite
+  import Msg = MessageHeader
+  import MessageBody
+  import Serialize
+  import Streams
+  import Signature
+  import Collections
+
+  // TODO This should probably implement a more generic Stream trait
+  class EncryptionStream {
+    ghost const Repr: set<object>
+    var producer: Collections.ByteProducer
+    // TODO If EncryptionStream implements a generic trait, this would have to be the generic
+    // ByteConsumer. However, we don't have a good way to get to the bits 'Accept'ed
+    // by a ByteConsumer. For now, explicitly use The EncryptionConsumer which
+    // has methods to get to the buffered bytes. I'm thinking that maybe
+    // we need to pipe two streams together, one which feeds bytes into the encryptor
+    // stream, and another which feeds from the encryptor to a ByteConsumer which is
+    // controlled by the extern (i.e. the extern could maintain the buffer of the extern 
+    // ByteConsumer and siphon from the encryptor to the extern ByteConsumer)
+    var consumer: EncryptionConsumer
+
+    predicate Valid()
+      reads this, Repr, this.consumer, this.producer, this.producer.Repr
+      ensures Valid() ==> this in Repr
+    {
+      && this.consumer.Valid()
+      && this.producer.Valid()
+      && this.consumer.Repr !! this.producer.Repr
+      && Repr == {this, consumer, producer}
+    }
+
+    constructor(producer: Collections.ByteProducer, consumer: EncryptionConsumer) {
+      this.Repr := {this, consumer, producer};
+      this.producer := producer;
+      this.consumer := consumer;
+    }
+
+    // TODO This is not the interface we want for getting bytes out of the stream.
+    // But is being used currently by shim ClientEncryptionStream to get to the
+    // encrypted bytes
+    // TODO this probably should return up to a count, not a single byte
+    method GetByte() returns (res: Result<Option<uint8>>)
+      requires Valid()
+      ensures Valid()
+      modifies producer, producer.Repr, consumer, consumer.Repr
+      decreases *
+    {
+      while !consumer.HasNext()
+        invariant Valid()
+        decreases *
+      {
+        // FIXME verifier is throwing a fit here over modifies clause
+        var siphoned :- producer.Siphon(consumer);
+        if siphoned == 0 {
+          // None means end of stream
+          return Success(None());
+        }
+      }
+      var nextByte :- consumer.Next();
+      return Success(Some(nextByte));
+    }
+  }
+
+  // Transforms plaintext into the encrypted message.
+  // Note that it is the consumer that is performing the transformation of the
+  // plaintext into the message. However, the requirement that we main both an
+  // input and output buffer here makes me think that this encapsulation
+  // isn't quite correct. Perhaps this logic needs to move entirely into the
+  // stream, and the consumer is just a way for the stream to define the
+  // buffer it is siphoning the input stream into and has access to.
+  class EncryptionConsumer extends Collections.ByteConsumer {
+    // TODO use ByteReader/Writer for these internal buffers?
+    // TODO I feel like we shouldn't need two buffers here
+    // This is a buffer to hold read plaintext which we have not encrypted yet.
+    var plaintext: seq<uint8>
+    // This is a buffer for the message which has been processed so far
+    var processedMessage: seq<uint8>
+    var header: Msg.HeaderBody
+    var dataKey: seq<uint8>
+    var encMat: Materials.EncryptionMaterials
+    var seqNum: uint32
+    // TODO Because I don't have a great way to figure out if we've reached
+    // the end of a stream, right now the logic for determining
+    // whether we're encrypting the final frame relies on knowing the
+    // total plaintextLength, and tracking how much we've encrypted so far.
+    // Note that this also requires that we know the total plaintext length
+    // before we begin, which requires either a seekable input stream
+    // or requires us to read the whole input into memory before beginning
+    var totalLength: int
+    var curLength: int
+    // TODO If we have signing right now we put the whole message in memory in
+    // order to sign it. There should be a better way to do this.
+    var toSign: seq<uint8>
+
+    predicate Valid() reads this ensures Valid() ==> this in Repr {
+      this in Repr
+    }
+
+    // TODO serHeader shouldn't be passed into constructor, but instead passed through the stream
+    constructor(serHeader: seq<uint8>, header: Msg.HeaderBody, dataKey: seq<uint8>, encMat: Materials.EncryptionMaterials, totalLength: int)
+      requires encMat.algorithmSuiteID.SignatureType().Some? ==> encMat.signingKey.Some?
+      requires |dataKey| == encMat.algorithmSuiteID.KeyLength()
+    {
+      this.plaintext := [];
+      this.processedMessage := serHeader;
+      this.header := header;
+      this.encMat := encMat;
+      this.dataKey := dataKey;
+      this.seqNum := 1;
+      this.totalLength := totalLength;
+      this.curLength := 0;
+      this.toSign := serHeader;
+      this.Repr := {this};
+    }
+
+    predicate method CanAccept() reads this, Repr
+      requires Valid()
+      ensures Valid()
+    {
+      curLength <= totalLength
+    }
+    
+    // Adds the accepted bit into our input buffer
+    // and if enough have been accumulated, process the
+    // plaintext into a frame in our output buffer
+    method Accept(b: uint8) returns (res: Result<()>)
+      requires Valid()
+      requires CanAccept()
+      ensures Valid()
+      modifies this, Repr
+    {
+      // Add to plaintext
+      plaintext := plaintext + [b];
+      // Update total Length
+      curLength := curLength + 1;
+      var frameLength := header.frameLength;
+
+      // TODO Split regular/final frame logic based on current position in input stream.
+      // I don't like this approach, but I think doing something like this is required
+      // as long as we do not have control over the number of bytes we are reading from
+      // input, and are instead "waiting" to accept some number. See above comment
+      // for moving encryption logic elsewhere.
+      if totalLength == curLength {
+        var frameToProcess := plaintext;
+        plaintext := [];
+        
+        var encryptedFrame :- MessageBody.EncryptFinalFrame(encMat.algorithmSuiteID, dataKey, frameLength as int, header.messageID, frameToProcess, seqNum);
+        processedMessage := processedMessage + encryptedFrame;
+        toSign := toSign + encryptedFrame;
+        // Since we've encrypted the final frame, we can also calculate
+        // the footer
+        var res :- AddSignatureToProcessedMessage();
+      } else if |plaintext| >= frameLength as int {
+        var frameToProcess := plaintext[..frameLength];
+        plaintext := plaintext[frameLength..];
+        var encryptedFrame :- MessageBody.EncryptRegularFrame(encMat.algorithmSuiteID, dataKey, frameLength as int, header.messageID, frameToProcess, seqNum);
+        processedMessage := processedMessage + encryptedFrame;
+        toSign := toSign + encryptedFrame;
+      }
+      return Success(());
+    }
+
+    method AddSignatureToProcessedMessage() returns (res: Result<bool>)
+      requires encMat.algorithmSuiteID.SignatureType().Some? ==> encMat.signingKey.Some?
+      modifies this`processedMessage
+    {
+      match encMat.algorithmSuiteID.SignatureType() {
+        case None =>
+        return Success(true);
+          // don't use a footer
+        case Some(ecdsaParams) =>
+          var digest :- Signature.Digest(ecdsaParams, toSign);
+          var bytes :- Signature.Sign(ecdsaParams, encMat.signingKey.get, digest);
+          if |bytes| != ecdsaParams.SignatureLength() as int {
+            return Failure("Malformed response from Sign().");
+          }
+          processedMessage := processedMessage + UInt16ToSeq(|bytes| as uint16) + bytes;
+          return Success(true);
+      }
+    }
+
+    predicate method HasNext()
+      reads this
+      requires Valid()
+      ensures Valid()
+    {
+      |processedMessage| > 0
+    }
+
+    method Next() returns (res: Result<uint8>) 
+      requires Valid()
+      //requires HasNext()
+      ensures Valid()
+      modifies this
+    {
+      // if we have stuff in the processedMessage. Take from that.
+      if |processedMessage| > 0 {
+        var byte := processedMessage[0];
+        // TODO will this grab correctly in the case that |processedMessage| == 1?
+        processedMessage := processedMessage[1..];
+        return Success(byte);
+      }
+    }
+  }
+}
